got notations working in OrderedType.v

theories/OrderedType.v
@@ -44,10 +44,22 @@ Record OrderedType : Type :=
  *** Commonly-Used Ordered Types
  ***)
 
+(* The ordered type of propositions *)
 Program Definition OTProp : OrderedType :=
   {|
     ot_Type := Prop;
     ot_R := iff;
+  |}.
+Next Obligation.
+  constructor.
+  { intros. transitivity y; assumption. }
+Qed.
+
+(* The ordered type of natural numbers *)
+Program Definition OTnat : OrderedType :=
+  {|
+    ot_Type := nat;
+    ot_R := le;
   |}.
 Next Obligation.
   constructor.
@@ -73,6 +85,7 @@ Program Definition OTType : OrderedType :=
   |}.
 *)
 
+(* The non-dependent function ordered type *)
 Program Definition OTArrow
             (A:OrderedType) (B: OrderedType) : OrderedType :=
   {|
@@ -90,17 +103,50 @@ Next Obligation.
   { apply H3; repeat split; assumption. }
 Qed.
 
-(*
-constructor.
-{ intro f; intros. apply (proj2_sig f). assumption. }
-{ intros f g h; intros.
-  apply (PreOrder_Transitive (PreOrder:=B) _ (proj1_sig g y)).
-  + apply H; assumption.
-  + apply H0; apply (PreOrder_Reflexive (PreOrder:=A) y). }
-Qed.
-*)
 
-(* FIXME: do product and sum types *)
+(* The non-dependent product ordered type *)
+Program Definition OTProd
+            (A:OrderedType) (B: OrderedType) : OrderedType :=
+  {|
+    ot_Type := ot_Type A * ot_Type B;
+    ot_R := fun p1 p2 =>
+              ot_R A (fst p1) (fst p2) /\ ot_R B (snd p1) (snd p2)
+  |}.
+Next Obligation.
+  constructor. intros p1 p2 p3; intros.
+  destruct H; destruct H0; destruct H1; destruct H2; destruct H3.
+  split.
+  { apply (semitransitivity (SemiTransitive:=A) _ (fst p2)); assumption. }
+  { apply (semitransitivity (SemiTransitive:=B) _ (snd p2)); assumption. }
+Qed.
+
+
+(* The non-dependent sum ordered type *)
+Program Definition OTSum
+            (A:OrderedType) (B: OrderedType) : OrderedType :=
+  {|
+    ot_Type := ot_Type A + ot_Type B;
+    ot_R := fun sum1 sum2 =>
+              match sum1, sum2 with
+                | inl x, inl y => ot_R A x y
+                | inl x, inr y => False
+                | inr x, inl y => False
+                | inr x, inr y => ot_R B x y
+              end
+  |}.
+Next Obligation.
+  constructor.
+  intros sum1 sum2 sum3; destruct sum1; destruct sum2; destruct sum3; intros.
+  { apply (semitransitivity (SemiTransitive:=A) _ o0); assumption. }
+  { assumption. }
+  { elimtype False; assumption. }
+  { elimtype False; assumption. }
+  { assumption. }
+  { elimtype False; assumption. }
+  { assumption. }
+  { apply (semitransitivity (SemiTransitive:=B) _ o0); assumption. }
+Qed.
+
 (* FIXME: also need notations *)
 
 (* FIXME: could also do a forall type, but need the second type argument, B, to
@@ -184,9 +230,9 @@ Inductive ContextExtends : OTContext -> OTContext -> Type :=
 .
 
 (* Context extension is reflexive *)
-Lemma ContextExtends_reflexive ctx : ContextExtends ctx ctx.
+Definition ContextExtends_reflexive ctx : ContextExtends ctx ctx.
   induction ctx; constructor; assumption.
-Qed.
+Defined.
 
 (* Context extension as a type class *)
 Class OTCtxExtends ctx1 ctx2 : Type :=
@@ -253,20 +299,20 @@ Qed.
  ***)
 
 (* Pairs of terms-in-context that are valid and related to each other *)
-Inductive OTPair ctx A : Type :=
-  mkOTPair (x1: ctx_elem ctx -> ot_Type A)
-           (x2: ctx_elem ctx -> ot_Type A)
-           (pf: validR (ot_R (OTInCtx ctx A)) x1 x2) :
-    OTPair ctx A.
+Inductive OTPairInCtx ctx A : Type :=
+  mkOTPairInCtx (x1: ctx_elem ctx -> ot_Type A)
+                (x2: ctx_elem ctx -> ot_Type A)
+                (pf: validR (ot_R (OTInCtx ctx A)) x1 x2) :
+    OTPairInCtx ctx A.
 
-(* Weakening the context of an OTPair *)
+(* Weakening the context of an OTPairInCtx *)
 Program Definition weaken_context {ctx1 ctx2} (ext: ContextExtends ctx1 ctx2)
-           {A} (p: OTPair ctx1 A) : OTPair ctx2 A :=
+           {A} (p: OTPairInCtx ctx1 A) : OTPairInCtx ctx2 A :=
   match p with
-    | mkOTPair _ _ x1 x2 pf =>
-      mkOTPair _ _ (fun celem1 => x1 (context_forget ext celem1))
-               (fun celem1 => x2 (context_forget ext celem1))
-               _
+    | mkOTPairInCtx _ _ x1 x2 pf =>
+      mkOTPairInCtx _ _ (fun celem1 => x1 (context_forget ext celem1))
+                    (fun celem1 => x2 (context_forget ext celem1))
+                    _
   end.
 Next Obligation.
   destruct pf as [ pf1 pf2 ]; destruct pf2 as [ pf2 pf3 ].
@@ -275,36 +321,9 @@ Next Obligation.
     apply context_forget_preserves_validR; assumption.
 Qed.
 
-
-(***
- *** Proper Terms
- ***)
-
-(* A "proper term" is an OTPair in the empty context *)
-Definition ProperTerm (A:OrderedType) := OTPair [] A.
-
-(* We can coerce a ProperTerm A to an element of ot_Type A by just taking the
-first projection of the pair in the ProperTerm *)
-Definition coerce_proper_term {A} (p: ProperTerm A) : ot_Type A :=
-  match p with
-  | mkOTPair _ _ x1 x2 pf => x1 tt
-  end.
-
-Coercion coerce_proper_term : ProperTerm >-> ot_Type.
-
-(* Any ProperTerm is always Proper *)
-Instance ProperTerm_Proper {A} (p:ProperTerm A) : Proper (ot_R A) p.
-destruct p; unfold coerce_proper_term. destruct pf; apply H.
-repeat split.
-Qed.
-
-
-(***
- *** Builders for Proper Terms using OTPair
- ***)
-
-Program Definition proper_var ctx A : OTPair (A::ctx) A :=
-  mkOTPair (A::ctx) A
+(* Build a term-in-context for the top-most variable in the context *)
+Program Definition top_var_in_context ctx A : OTPairInCtx (A::ctx) A :=
+  mkOTPairInCtx (A::ctx) A
            (fun ctx_elem =>
               let (celem_A,_) := ctx_elem in celem_A)
            (fun ctx_elem =>
@@ -318,14 +337,99 @@ Next Obligation.
           assumption.
 Qed.
 
+(* OTPairInCtx is a functor w.r.t. proper functions *)
+Program Definition map_OTPairInCtx {ctx A B}
+        (f: ot_Type A -> ot_Type B)
+        (proper: Proper (validR (ot_R A) ==> validR (ot_R B)) f)
+        (x: OTPairInCtx ctx A) : OTPairInCtx ctx B :=
+  let (x1,x2,pf_x) := x in
+  mkOTPairInCtx _ _ (fun celem => f (x1 celem)) (fun celem => f (x2 celem)) _.
+Next Obligation.
+  destruct pf_x as [ pfx_1 pfx_2 ]; destruct pfx_2 as [ pfx_2 pfx_3 ].
+  repeat split; intros celem1 celem2 H; apply proper; repeat split;
+  first [ apply pfx_1 | apply pfx_2 | apply pfx_3 ];
+  try assumption; destruct H; destruct H0; repeat split; assumption.
+Qed.
+
+(* OTPairInCtx is also a bi-functor w.r.t. proper functions *)
+Program Definition map2_OTPairInCtx {ctx A B C}
+        (f: ot_Type A -> ot_Type B -> ot_Type C)
+        (proper: Proper (validR (ot_R A) ==> validR (ot_R B) ==> validR (ot_R C)) f)
+        (x: OTPairInCtx ctx A) (y: OTPairInCtx ctx B) : OTPairInCtx ctx C :=
+  let (x1,x2,pf_x) := x in
+  let (y1,y2,pf_y) := y in
+  mkOTPairInCtx _ _ (fun celem => f (x1 celem) (y1 celem))
+                (fun celem => f (x2 celem) (y2 celem)) _.
+Next Obligation.
+  destruct pf_x as [ pfx_1 pfx_2 ]; destruct pfx_2 as [ pfx_2 pfx_3 ].
+  destruct pf_y as [ pfy_1 pfy_2 ]; destruct pfy_2 as [ pfy_2 pfy_3 ].
+  repeat split; intros celem1 celem2 H; apply proper; repeat split;
+  first [ apply pfx_1 | apply pfy_1 | apply pfx_2 | apply pfy_2 |
+          apply pfx_3 | apply pfy_3 ];
+  try assumption; destruct H; destruct H0; repeat split; assumption.
+Qed.
+
+(* OTPairInCtx is also a tri-functor w.r.t. proper functions *)
+Program Definition map3_OTPairInCtx {ctx A B C D}
+        (f: ot_Type A -> ot_Type B -> ot_Type C -> ot_Type D)
+        (proper: Proper (validR (ot_R A) ==> validR (ot_R B) ==>
+                                validR (ot_R C) ==> validR (ot_R D)) f)
+        (x: OTPairInCtx ctx A) (y: OTPairInCtx ctx B) (z: OTPairInCtx ctx C)
+: OTPairInCtx ctx D :=
+  let (x1,x2,pf_x) := x in
+  let (y1,y2,pf_y) := y in
+  let (z1,z2,pf_z) := z in
+  mkOTPairInCtx _ _ (fun celem => f (x1 celem) (y1 celem) (z1 celem))
+                (fun celem => f (x2 celem) (y2 celem) (z2 celem)) _.
+Next Obligation.
+  destruct pf_x as [ pfx_1 pfx_2 ]; destruct pfx_2 as [ pfx_2 pfx_3 ].
+  destruct pf_y as [ pfy_1 pfy_2 ]; destruct pfy_2 as [ pfy_2 pfy_3 ].
+  destruct pf_z as [ pfz_1 pfz_2 ]; destruct pfz_2 as [ pfz_2 pfz_3 ].
+  repeat split; intros celem1 celem2 H; apply proper; repeat split;
+  first [ apply pfx_1 | apply pfy_1 | apply pfz_1 |
+          apply pfx_2 | apply pfy_2 | apply pfz_2 |
+          apply pfx_3 | apply pfy_3 | apply pfz_3 ];
+  try assumption; destruct H; destruct H0; repeat split; assumption.
+Qed.
+
+
+(***
+ *** Top-Level Proper Terms
+ ***)
+
+(* A "proper term" is an OTPairInCtx in the empty context *)
+Definition ProperTerm (A:OrderedType) := OTPairInCtx [] A.
+
+(* We can coerce a ProperTerm A to an element of ot_Type A by just taking the
+first projection of the pair in the ProperTerm *)
+Definition coerce_proper_term {A} (p: ProperTerm A) : ot_Type A :=
+  match p with
+  | mkOTPairInCtx _ _ x1 x2 pf => x1 tt
+  end.
+
+Coercion coerce_proper_term : ProperTerm >-> ot_Type.
+
+(* Any ProperTerm is always Proper *)
+Instance ProperTerm_Proper {A} (p:ProperTerm A) : Proper (ot_R A) p.
+destruct p; unfold coerce_proper_term. destruct pf; apply H.
+repeat split.
+Qed.
+
+
+(***
+ *** Builders for Proper Terms using OTPairInCtx
+ ***)
+
+(* Helper to build a ProperTerm for a function *)
 Program Definition proper_fun {ctx} {A} {B}
-        (f: (forall {ctx'} `{ext: OTCtxExtends (A::ctx) ctx'}, OTPair ctx' A) ->
-            OTPair (A::ctx) B) :
-  OTPair ctx (OTArrow A B) :=
+        (f: (forall {ctx'} `{ext: OTCtxExtends (A::ctx) ctx'},
+               OTPairInCtx ctx' A) ->
+            OTPairInCtx (A::ctx) B) :
+  OTPairInCtx ctx (OTArrow A B) :=
   let (y1,y2,pf_y) :=
-      f (fun {ctx'} {ext} => weaken_context ext (proper_var ctx A))
+      f (fun {ctx'} {ext} => weaken_context ext (top_var_in_context ctx A))
   in
-  mkOTPair _ _ (fun ctx_elem x => y1 (x,ctx_elem))
+  mkOTPairInCtx _ _ (fun ctx_elem x => y1 (x,ctx_elem))
            (fun ctx_elem x => y2 (x,ctx_elem)) _.
 Next Obligation.
   destruct pf_y as [ pf1 pf2 ]; destruct pf2 as [ pf2 pf3 ].
@@ -333,28 +437,193 @@ Next Obligation.
   apply ctx_elem_lt_cons; assumption.
 Qed.
 
+(* Helper to implicitly add the arguments for a ProperTerm variable *)
+Definition proper_var {ctx} {A}
+           (var: (forall ctx' (ext: OTCtxExtends (A::ctx) ctx'),
+                    OTPairInCtx ctx' A))
+           {ctx'} {ext: OTCtxExtends (A::ctx) ctx'} :
+  OTPairInCtx ctx' A :=
+  var ctx' ext.
+
+
+(* Helper to build a ProperTerm for an application *)
+Program Definition proper_apply {ctx} {A} {B}
+        (f: OTPairInCtx ctx (OTArrow A B))
+        (x: OTPairInCtx ctx A) : OTPairInCtx ctx B :=
+  map2_OTPairInCtx (A:=OTArrow A B) (fun g y => g y) _ f x.
+Next Obligation.
+  intros f1 f2 pf_f;
+  destruct pf_f as [ pf_f1 pf_f2 ]; destruct pf_f2 as [ pf_f2 pf_f3 ];
+  intros x1 x2 pf_x;
+  destruct pf_x as [ pf_x1 pf_x2 ]; destruct pf_x2 as [ pf_x2 pf_x3 ];
+  repeat split;
+  first [ apply pf_f1 | apply pf_f2 | apply pf_f3 ];
+  repeat split; assumption.
+Qed.
+
+(* Helper to build a ProperTerm for a pair *)
+Program Definition proper_pair {ctx} {A} {B}
+           (x: OTPairInCtx ctx A) (y: OTPairInCtx ctx B) :
+  OTPairInCtx ctx (OTProd A B) :=
+  map2_OTPairInCtx (C:=OTProd A B) (fun x y => (x,y)) _ x y.
+Next Obligation.
+repeat (intro; intros); destruct H; destruct H1; destruct H0; destruct H3.
+unfold fst, snd; repeat split; assumption.
+Qed.
+
+(* Helper to build a ProperTerm for a first projection *)
+Program Definition proper_proj1 {ctx} {A} {B}
+           (x: OTPairInCtx ctx (OTProd A B)) : OTPairInCtx ctx A :=
+  map_OTPairInCtx (A:=OTProd A B) (fun p => fst p) _ x.
+Next Obligation.
+  intros p1 p2; destruct p1; destruct p2; unfold fst;
+  intro pf_p; destruct pf_p.
+  destruct H; repeat destruct H0; destruct H2.
+  repeat split; assumption.
+Qed.
+
+(* Helper to build a ProperTerm for a second projection *)
+Program Definition proper_proj2 {ctx} {A} {B}
+           (x: OTPairInCtx ctx (OTProd A B)) : OTPairInCtx ctx B :=
+  map_OTPairInCtx (A:=OTProd A B) (fun p => snd p) _ x.
+Next Obligation.
+  intros p1 p2; destruct p1; destruct p2; unfold snd;
+  intro pf_p; destruct pf_p.
+  destruct H; repeat destruct H0; destruct H2.
+  repeat split; assumption.
+Qed.
+
+(* Helper to build a ProperTerm for the inl constructor *)
+Program Definition proper_inl {ctx} {A} {B}
+           (x: OTPairInCtx ctx A) : OTPairInCtx ctx (OTSum A B) :=
+  map_OTPairInCtx (B:=OTSum A B) (fun y => inl y) _ x.
+Next Obligation.
+  intros x1 x2 pf_x; assumption.
+Qed.
+
+(* Helper to build a ProperTerm for the inr constructor *)
+Program Definition proper_inr {ctx} {A} {B}
+           (x: OTPairInCtx ctx B) : OTPairInCtx ctx (OTSum A B) :=
+  map_OTPairInCtx (B:=OTSum A B) (fun y => inr y) _ x.
+Next Obligation.
+  intros x1 x2 pf_x; assumption.
+Qed.
+
+(* Helper to build a ProperTerm for sum elimination *)
+Program Definition proper_sum_elim {ctx} {A} {B} {C}
+           (x: OTPairInCtx ctx (OTSum A B))
+           (f1: OTPairInCtx ctx (OTArrow A C))
+           (f2: OTPairInCtx ctx (OTArrow B C))
+: OTPairInCtx ctx C :=
+  map3_OTPairInCtx (A:=OTSum A B) (B:=OTArrow A C) (C:=OTArrow B C)
+                   (fun y g1 g2 => match y with
+                                     | inl y1 => g1 y1
+                                     | inr y2 => g2 y2
+                                   end) _ x f1 f2.
+Next Obligation.
+  intros sum1 sum2; destruct sum1; destruct sum2;
+  intros H g1 g2 pf_g h1 h2 pf_h; destruct H; destruct H0;
+  destruct pf_g as [ pf_g1 pf_g2 ]; destruct pf_g2 as [ pf_g2 pf_g3 ];
+  destruct pf_h as [ pf_h1 pf_h2 ]; destruct pf_h2 as [ pf_h2 pf_h3 ];
+  repeat split;
+  first [ apply pf_g1 | apply pf_g2 | apply pf_g3
+          | apply pf_h1 | apply pf_h2 | apply pf_h3
+          | elimtype False; assumption ];
+  repeat split; assumption.
+Qed.
+
+
+(***
+ *** Notations
+ ***)
+
+Module ProperTermNotations.
+
+  Notation "A '-o>' B" :=
+    (OTArrow A B) (right associativity, at level 99).
+  Notation "A '*o*' B" :=
+    (OTProd A B) (left associativity, at level 40).
+  Notation "A '+o+' B" :=
+    (OTSum A B) (left associativity, at level 50).
+
+  Delimit Scope pterm_scope with pterm.
+
+  Bind Scope pterm_scope with ProperTerm.
+
+  Notation "'pfun' ( x ::: T ) ==> y" :=
+    (proper_fun (A:=T) (fun x => y%pterm))
+      (at level 100, right associativity, x at level 99) : pterm_scope.
+
+  Notation "'pvar' x" := (proper_var x) (no associativity, at level 75) : pterm_scope.
+
+  Notation "x @ y" :=
+    (proper_apply x y) (right associativity, at level 20) : pterm_scope.
+
+  Notation "( x ,o, y )" :=
+    (proper_pair x%pterm y%pterm)
+      (no associativity, at level 0) : pterm_scope.
+  Notation "'ofst' x" :=
+    (proper_proj1 x%pterm) (right associativity, at level 80) : pterm_scope.
+  Notation "'osnd' x" :=
+    (proper_proj2 x%pterm) (right associativity, at level 80) : pterm_scope.
+
+  Notation "'pinl' ( B ) x" :=
+    (proper_inl (B:=B) x) (right associativity, at level 80) : pterm_scope.
+  Notation "'pinr' ( A ) x" :=
+    (proper_inl (A:=A) x) (right associativity, at level 80) : pterm_scope.
+  Notation "'pmatch_sum' x 'with' | 'inl' y1 => z1 | 'inr' y2 => z2 'end'" :=
+    (proper_sum_elim x (proper_fun (fun y1 => z1))
+                     (proper_fun (fun y2 => z2)))
+      (no associativity, at level 0, x at level 100).
+
+  (* NOTE: this notation needs to be in a Program Instance *)
+  Notation "'pmap1' ( f ::: A --> B ) x" :=
+    (map_OTPairInCtx (A:=A) (B:=B) f _ x)
+      (right associativity, at level 80) : pterm_scope.
+
+End ProperTermNotations.
+
 
 (***
  *** Examples
  ***)
 
-(* Example: the identity on Prop *)
-Definition proper_id_Prop_fun : ProperTerm (OTArrow OTProp OTProp) :=
-  proper_fun (A:=OTProp) (fun x => x _ _).
+Module ProperTermExamples.
 
-(* It is the identity, and we get an automatic Proper proof for it *)
+Import ProperTermNotations.
+
+(* Example: the identity on Prop *)
+Definition proper_id_Prop_fun : ProperTerm (OTProp -o> OTProp) :=
+  pfun ( x ::: OTProp ) ==> pvar x.
+
+(* You can see that it yields the identity function *)
 Eval compute in (coerce_proper_term proper_id_Prop_fun : Prop -> Prop).
-Goal (Proper (OTArrow OTProp OTProp) proper_id_Prop_fun).
+
+(* The proof of Proper-ness is automatic by typeclass instances *)
+Goal (Proper (OTProp -o> OTProp) proper_id_Prop_fun).
 auto with typeclass_instances.
 Qed.
 
 (* Example 2: the first projection function on 2 Props *)
-Definition proper_proj1_Prop_fun : ProperTerm (OTArrow OTProp (OTArrow OTProp OTProp)) :=
-  proper_fun (A:=OTProp)
-             (fun x =>
-                (proper_fun (A:=OTProp) (fun y => x _ _))).
+Definition proper_proj1_Prop_fun : ProperTerm (OTProp -o> OTProp -o> OTProp) :=
+  pfun ( P1 ::: OTProp ) ==>
+    pfun ( P2 ::: OTProp ) ==>
+      pvar P1.
 
-Eval compute in (coerce_proper_term proper_proj1_Prop_fun).
-Goal (Proper (OTArrow OTProp (OTArrow OTProp OTProp)) proper_proj1_Prop_fun).
-auto with typeclass_instances.
-Qed.
+(* Example 3: apply each of a pair of functions to an argument *)
+Definition proper_example3 {A B C} :
+  ProperTerm ((A -o> B) *o* (A -o> C) -o> A -o> (B *o* C)) :=
+  pfun ( p ::: (A -o> B) *o* (A -o> C)) ==>
+    pfun ( x ::: A ) ==>
+      (((ofst (pvar p)) @ pvar x) ,o, ((osnd (pvar p)) @ pvar x)).
+
+(* Example 4: match a sum of two A's and return an A *)
+Definition proper_example4 {A} :
+  ProperTerm (A +o+ A -o> A) :=
+  pfun ( sum ::: A +o+ A) ==>
+    pmatch_sum (pvar sum) with
+      | inl x => pvar x
+      | inr y => pvar y
+    end.
+
+End ProperTermExamples.
